redid readme and started sanytising

theories/iris/examples/effects/wat-code/client.wat
@@ -1,0 +1,33 @@
+;; run with the specfx fork of the reference interpreter with
+;; ./wasm coroutine.wat -e '(module instance)' -e '(register "coroutine")' client.wat -e '(module instance)' -e '(invoke "main")'
+;; it should display
+;; [0 42] : [i32 i32]
+(module ;; client
+  (type $func (func))
+  (import "coroutine" "yield" (func $yield)) ;; needs yield and par
+  (import "coroutine" "par" (func $par (param (ref $func)) (param (ref $func))))
+  (global $x (mut i32) (i32.const 0))        ;; shared `data' $x
+  (global $y (mut i32) (i32.const 0))        ;; shared `flag' $y
+  (global $a (mut i32) (i32.const 0))        ;; reader's copy of the value of $y
+  (global $b (mut i32) (i32.const 0))        ;; reader's copy of the value of $x
+  (elem declare funcref (ref.func $f1))      ;; make $f1 available
+  (elem declare funcref (ref.func $f2))      ;; and $f2
+  (func $f1
+    i32.const 42                             ;; write 42 to $x
+    global.set $x
+    call $yield                              ;; yield
+    i32.const 1                              ;; set the flag
+    global.set $y)
+  (func $f2
+    global.get $y                            ;; read from $y
+    global.set $a                            ;; save in $a
+    call $yield                              ;; yield
+    global.get $x                            ;; read from $x
+    global.set $b)                           ;; save in $b
+  (func $main (result i32 i32)
+    ref.func $f1                             ;; run $f1 and $f2 concurrently
+    ref.func $f2
+    call $par
+    global.get $a                            ;; look up what the reader saw
+    global.get $b)
+  (export "main" (func $main)))              ;; make $main available outside
