theories/iris/helpers/reduce_det/reduce_det_local_const.v
@@ -20,8 +20,6 @@ Proof.
   all: try by inversion Heqves'.
   all: try by do 4 destruct vs0 => //.
   all: try by do 4 destruct vcs => //.
-(*  - inversion Heqves'; subst. repeat split => //. done. *)
-(*  - inversion Heqves'; subst => //. *)
   - inversion Heqves'; subst.
     apply lfilled_const in H2 as [??] => //.
     apply const_list_split in H2 as [??] => //.
@@ -60,8 +58,6 @@ Proof.
   all: try by inversion Heqves'.
   all: try by do 4 destruct vs => //.
   all: try by do 4 destruct vcs => //.
-(*  - inversion Heqves'; subst => //. 
-  - inversion Heqves'; subst; repeat split => //.  *)
   - inversion Heqves'; subst.
     eapply filled_singleton in H2 as (_ & _ & ?) => //.
     all: do 2 destruct e' => //.
