theories/iris/examples/effects/wat-code/README.md
@@ -1,0 +1,3 @@
+A coroutine example.
+See the client file for instructions to run using the extended reference interpreter from
+https://github.com/wasmfx/specfx
